dimsum/iris/language.v
@@ -1,0 +1,43 @@
+From iris.program_logic Require Export language.
+From iris.program_logic Require Import weakestpre.
+From dimsum.core.iris Require Export sim.
+Set Default Proof Using "Type".
+
+Definition nb_step EV (_ : unit) (_ : option EV) (_ : unit → Prop) : Prop := False.
+Definition nb_trans EV : mod_trans EV := ModTrans (nb_step EV).
+Canonical Structure nb_mod_lang EV : mod_lang EV := {|
+  mexpr := unit;
+  mtrans := nb_trans EV;
+  mexpr_rel _ _ := True;
+|}.
+
+Inductive lang_step (Λ : language) :
+  (expr Λ * state Λ) → option (observation Λ) → ((expr Λ * state Λ) → Prop) → Prop :=
+| LangStep e σ e' σ' efs κs :
+  prim_step e σ κs e' σ' efs →
+  lang_step Λ (e, σ) (head κs) (λ σ'', σ'' = (e', σ')).
+
+Definition lang_trans (Λ : language) : mod_trans (observation Λ) :=
+  ModTrans (lang_step Λ).
+
+Canonical Structure lang_mod_lang (Λ : language) : mod_lang (observation Λ) := {|
+  mexpr := expr Λ;
+  mtrans := lang_trans Λ;
+  mexpr_rel σ e := e = σ.1;
+|}.
+
+Section wp.
+  Context {Λ : language}.
+  Context `{!irisGS_gen HasNoLc Λ Σ}.
+
+  Lemma sim_wp_adequacy e E Φ `{!ord_laterPreG Σ}:
+    (∀ γ_ord,
+      let _ : ord_laterGS Σ := OrdLaterGS _ _ γ_ord in
+      ∃ (stateI : (lang_trans Λ).(m_state) → (nb_trans _).(m_state) → iProp Σ),
+      (* TODO: Add a proof that the two state interpretations coincide. *)
+      let _ : dimsumGS _ (lang_mod_lang Λ) (nb_mod_lang _) Σ := DimsumGS _ _ _ _ _ _ stateI in
+     e ⪯{E} tt {{ λ e _, ∃ v, ⌜to_val e = Some v⌝ ∗ Φ v }}) -∗
+    WP e @ E {{ Φ }}.
+  Proof.
+  Abort.
+End wp.
